rupicola/io/Backtranslation.fsti
@@ -10,4 +10,4 @@ val typing : typ_env -> exp -> qType -> Type u#1
 val backtranslate (#g:typ_env) (#e:exp) (#t:qType) (h:typing g e t) (fs_g:eval_env g) : (get_Type t)
 
 val lem_backtranslate #g (#e:exp{fv_in_env g e}) #t (h:typing g e t) : Lemma
-(equiv_oval t (backtranslate h) e)
+(backtranslate h ≈ e)
