rupicola/io/Compilation.fsti
@@ -13,10 +13,10 @@ val lem_compile_empty_closed #a (#s:fs_oval empty a) (qs:empty ⊢ s) : Lemma (i
 
 val compile_closed (#a:qType) (#s:get_Type a) (qs:a ⊩ s) : closed_exp
 val compile_equiv #g (#a:qType) (#s:fs_oval g a) (qs:g ⊢ s)
-  : Lemma (ensures (s `equiv_oval a` (compile qs))) (decreases qs)
+  : Lemma (ensures (s ≈ (compile qs))) (decreases qs)
 
 val compile_closed_equiv (#a:qType) (#s:get_Type a) (qs:a ⊩ s)
   : Lemma (ensures (forall h. a ⦂ (h, s, compile_closed qs)))
 
-val lemma_compile_closed_arrow_is_elam (#a #b:qType) (#s:fs_val (a ^-> b)) (qs: (a ^-> b) ⊩ s)
+val lemma_compile_closed_arrow_is_elam (#a #b:qType) (#s:fs_val (a ^->!@ b)) (qs: (a ^->!@ b) ⊩ s)
   : Lemma (ELam? (compile_closed qs))
